rewrite ~~in rust~~ to the new ValidPos api

src/Lean/Compiler/NameMangling.lean
@@ -52,44 +52,72 @@ end String
 
 namespace Lean
 
-private def checkLowerHex : Nat → String → String.Pos.Raw → Bool
+private def checkLowerHex : Nat → (s : String) → s.ValidPos → Bool
   | 0, _, _ => true
   | k + 1, s, pos =>
-    if h : s.atEnd pos then
+    if h : pos = s.endValidPos then
       false
     else
-      let ch := s.get' pos h
+      let ch := pos.get h
       (ch.isDigit || (ch.val >= 97 && ch.val <= 102)) && -- 0-9a-f
-        checkLowerHex k s (s.next' pos h)
+        checkLowerHex k s (pos.next h)
 
-private def parseLowerHex : Nat → String → String.Pos.Raw → Nat → Nat
-  | 0, _, _, n => n
-  | k + 1, s, pos, n =>
-    let ch := s.get pos
-    let pos := s.next pos
-    if ch.isDigit then parseLowerHex k s pos (n <<< 4 ||| (ch.val - 48).toNat)
-    else parseLowerHex k s pos (n <<< 4 ||| (ch.val - 87).toNat)
+private theorem valid_of_checkLowerHex (h : checkLowerHex n s p) :
+    (String.Pos.Raw.mk (p.offset.byteIdx + n)).IsValid s := by
+  fun_induction checkLowerHex
+  · rename_i p
+    exact p.isValid
+  · contradiction
+  · rename_i k s p hp ch ih
+    simp only [Bool.and_eq_true, Bool.or_eq_true, decide_eq_true_eq] at h
+    specialize ih h.2
+    refine cast ?_ ih
+    congr 2
+    simp only [String.ValidPos.next, String.Slice.Pos.ofset_ofSlice,
+      String.Slice.Pos.byteIdx_offset_next, String.ValidPos.offset_toSlice, Nat.succ_eq_add_one]
+    change p.offset.byteIdx + ch.utf8Size + k = _
+    rw [Char.utf8Size_eq_one_iff.mpr, Nat.add_assoc, Nat.add_comm 1]
+    rcases h.1 with h | h
+    · simp only [Char.isDigit, Bool.and_eq_true, decide_eq_true_eq] at h
+      exact UInt32.le_trans h.2 (by decide)
+    · exact UInt32.le_trans h.2 (by decide)
 
-private def checkDisambiguation : Nat → String → String.Pos.Raw → Bool
+private def parseLowerHex : (n : Nat) → (s : String) → (p : s.ValidPos) →
+    checkLowerHex n s p → Nat → Nat
+  | 0, _, _, _, n => n
+  | k + 1, s, pos, h, n =>
+    have hpos : pos ≠ s.endValidPos := by
+      rw [checkLowerHex] at h
+      split at h <;> trivial
+    let ch := pos.get hpos
+    let pos := pos.next hpos
+    have h' : checkLowerHex k s pos := by
+      simp only [checkLowerHex, hpos, ↓reduceDIte, ge_iff_le, Bool.and_eq_true, Bool.or_eq_true,
+        decide_eq_true_eq, pos] at h ⊢
+      exact h.2
+    if ch.isDigit then parseLowerHex k s pos h' (n <<< 4 ||| (ch.val - 48).toNat)
+    else parseLowerHex k s pos h' (n <<< 4 ||| (ch.val - 87).toNat)
+
+private def checkDisambiguation : Nat → (s : String) → s.ValidPos → Bool
   | 0, _, _ => true
   | k + 1, s, p =>
     if h : _ then
-      let b := s.getUTF8Byte p h
-      if b = '_'.toUInt8 then
-        checkDisambiguation k s ⟨p.byteIdx + 1⟩
-      else if b = 'x'.toUInt8 then
-        checkLowerHex 2 s ⟨p.byteIdx + 1⟩
-      else if b = 'u'.toUInt8 then
-        checkLowerHex 4 s ⟨p.byteIdx + 1⟩
-      else if b = 'U'.toUInt8 then
-        checkLowerHex 8 s ⟨p.byteIdx + 1⟩
-      else if b >= 48 && b <= 57 then
+      let b := p.get h
+      if b = '_' then
+        checkDisambiguation k s (p.next h)
+      else if b = 'x' then
+        checkLowerHex 2 s (p.next h)
+      else if b = 'u' then
+        checkLowerHex 4 s (p.next h)
+      else if b = 'U' then
+        checkLowerHex 8 s (p.next h)
+      else if b.val >= 48 && b.val <= 57 then
         true
       else false
     else true
 
 private def needDisambiguation (prev : String) (next : String) : Bool :=
-  prev.endsWith "__" || checkDisambiguation next.utf8ByteSize next 0
+  prev.endsWith "__" || checkDisambiguation next.utf8ByteSize next next.startValidPos
 
 private def Name.mangleAux : Name → String
   | Name.anonymous => ""
@@ -97,7 +125,7 @@ private def Name.mangleAux : Name → String
     let m := String.mangle s
     match p with
     | Name.anonymous =>
-      if checkDisambiguation m.utf8ByteSize m 0 then "00" ++ m else m
+      if checkDisambiguation m.utf8ByteSize m m.startValidPos then "00" ++ m else m
     | p              =>
       let m1 := mangleAux p
       m1 ++ (if needDisambiguation m1 m then "_00" else "_") ++ m
@@ -116,55 +144,55 @@ def mkModuleInitializationFunctionName (moduleName : Name) : String :=
   "initialize_" ++ moduleName.mangle ""
 
 -- assumes `s` has been generated `Name.mangle n ""`
-private def Name.unmangleAux (s : String) (p : String.Pos.Raw) (res : Name)
+private def Name.unmangleAux (s : String) (p : s.ValidPos) (res : Name)
     (acc : String) (ucount : Nat) : Nat → Name
   | 0 => res.str (acc.pushn '_' (ucount / 2))
   | k + 1 =>
-    if h : s.atEnd p then res.str (acc.pushn '_' (ucount / 2)) else
-    let ch := s.get' p h
-    let p := s.next' p h
+    if h : p = s.endValidPos then res.str (acc.pushn '_' (ucount / 2)) else
+    let ch := p.get h
+    let p := p.next h
     if ch = '_' then unmangleAux s p res acc (ucount + 1) k else
     if ucount % 2 = 0 then
       unmangleAux s p res (acc.pushn '_' (ucount / 2) |>.push ch) 0 k
     else if ch.isDigit then
       let res := res.str (acc.pushn '_' (ucount / 2))
-      if ch = '0' ∧ s.get p = '0' then
-        unmangleAux s (s.next p) res "" 0 k
+      if h : ch = '0' ∧ ∃ h : p ≠ s.endValidPos, p.get h = '0' then
+        unmangleAux s (p.next h.2.1) res "" 0 k
       else
         decodeNum s p res (ch.val - 48).toNat k
-    else if ch = 'x' ∧ checkLowerHex 2 s p then
+    else if h : ch = 'x' ∧ checkLowerHex 2 s p then
       let acc := acc.pushn '_' (ucount / 2)
-      unmangleAux s ⟨p.byteIdx + 2⟩ res (acc.push (Char.ofNat (parseLowerHex 2 s p 0))) 0 k
-    else if ch = 'u' ∧ checkLowerHex 4 s p then
+      unmangleAux s ⟨_, valid_of_checkLowerHex h.2⟩ res (acc.push (Char.ofNat (parseLowerHex 2 s p h.2 0))) 0 k
+    else if h : ch = 'u' ∧ checkLowerHex 4 s p then
       let acc := acc.pushn '_' (ucount / 2)
-      unmangleAux s ⟨p.byteIdx + 4⟩ res (acc.push (Char.ofNat (parseLowerHex 4 s p 0))) 0 k
-    else if ch = 'U' ∧ checkLowerHex 8 s p then
+      unmangleAux s ⟨_, valid_of_checkLowerHex h.2⟩ res (acc.push (Char.ofNat (parseLowerHex 4 s p h.2 0))) 0 k
+    else if h : ch = 'U' ∧ checkLowerHex 8 s p then
       let acc := acc.pushn '_' (ucount / 2)
-      unmangleAux s ⟨p.byteIdx + 8⟩ res (acc.push (Char.ofNat (parseLowerHex 8 s p 0))) 0 k
+      unmangleAux s ⟨_, valid_of_checkLowerHex h.2⟩ res (acc.push (Char.ofNat (parseLowerHex 8 s p h.2 0))) 0 k
     else
       unmangleAux s p (res.str acc) ("".pushn '_' (ucount / 2) |>.push ch) 0 k
 where
-  decodeNum (s : String) (p : String.Pos.Raw) (res : Name) (n : Nat) : Nat → Name
+  decodeNum (s : String) (p : s.ValidPos) (res : Name) (n : Nat) : Nat → Name
     | 0 => res.num n
     | k + 1 =>
-      if h : s.atEnd p then res.num n else
-      let ch := s.get' p h
-      let p := s.next' p h
+      if h : p = s.endValidPos then res.num n else
+      let ch := p.get h
+      let p := p.next h
       if ch.isDigit then
         decodeNum s p res (n * 10 + (ch.val - 48).toNat) k
       else -- assume ch = '_'
         let res := res.num n
-        if h : s.atEnd p then res else
-        nameStart s (s.next' p h) res k -- assume s.get' p h = '_'
-  nameStart (s : String) (p : String.Pos.Raw) (res : Name) : Nat → Name
+        if h : p = s.endValidPos then res else
+        nameStart s (p.next h) res k -- assume s.get' p h = '_'
+  nameStart (s : String) (p : s.ValidPos) (res : Name) : Nat → Name
     | 0 => res
     | k + 1 =>
-      if h : s.atEnd p then res else
-      let ch := s.get' p h
-      let p := s.next' p h
+      if h : p = s.endValidPos then res else
+      let ch := p.get h
+      let p := p.next h
       if ch.isDigit then
-        if ch = '0' ∧ s.get p = '0' then
-          unmangleAux s (s.next p) res "" 0 k
+        if h : ch = '0' ∧ ∃ h : p ≠ s.endValidPos, p.get h = '0' then
+          unmangleAux s (p.next h.2.1) res "" 0 k
         else
           decodeNum s p res (ch.val - 48).toNat k
       else if ch = '_' then
@@ -173,7 +201,7 @@ where
         unmangleAux s p res (String.singleton ch) 0 k
 
 def Name.unmangle (s : String) : Name :=
-  unmangleAux.nameStart s 0 .anonymous s.length
+  unmangleAux.nameStart s s.startValidPos .anonymous s.length
 
 def Name.unmangle? (s : String) : Option Name :=
   let n := unmangle s
